GraphProblems

CODIGO/GRAFOS/Problems/CliqueProblem.dfy
@@ -1,10 +1,8 @@
-include "../Auxiliar/Node.dfy"
+include "../Auxiliar/Graph.dfy"
 
-ghost predicate Clique(graph : set<Node>, k:int)
-reads graph
+ghost predicate Clique(graph:Graph, k:int)
 {
-  var A: set<set<Node>> := (set node, adj | node in graph && adj in node.adyacentes:: {node, adj});
-  exists s:set<Node> :: isClique(s,A) && |s| >= k && s <= graph
+  exists s:set<Node> :: isClique(s,graph.1) && |s| >= k && s <= graph.0
 }
 
 ghost predicate isClique(s:set<Node>, A:set<set<Node>>)
