CODIGO/GRAFOS/Transformations/IndependentSetToVertexCover.dfy
@@ -1,0 +1,36 @@
+include "../Auxiliar/Graph.dfy"
+include "../Problems/IndependentSet.dfy"
+include "../Problems/VertexCover.dfy"
+
+function IndependentSet_to_VertexCover(graph:Graph, k:int) : (r:(Graph,int))
+{
+    (graph,|graph.0|-k)
+}
+
+lemma IndependentSet_VertexCover(graph:Graph, k:int)
+  ensures var (Vgraph,Vk):= IndependentSet_to_VertexCover(graph,k);
+          IndependentSet(graph,k) <==> IndependentSet(Vgraph,Vk)
+{ 
+    IndependentSet_VertexCover1(graph,k);
+    IndependentSet_VertexCover2(graph,k);
+}
+
+lemma IndependentSet_VertexCover1(graph:Graph, k:int)
+    ensures var (Vgraph,Vk) := IndependentSet_to_VertexCover(graph,k);
+          IndependentSet(graph,k) <== VertexCover(Vgraph,Vk)
+{   
+    var (Vgraph,Vk) := IndependentSet_to_VertexCover(graph,k);
+    if (VertexCover(Vgraph,Vk)) {
+        
+    }
+}
+
+lemma IndependentSet_VertexCover2(graph:Graph, k:int)
+    ensures var (Vgraph,Vk) := IndependentSet_to_VertexCover(graph,k);
+          IndependentSet(graph,k) ==> VertexCover(Vgraph,Vk)
+{
+
+    if (IndependentSet(graph,k)) {
+        
+    }
+}
